Transducer.v
@@ -109,4 +109,37 @@ Definition body_td A := exists (L: aset), ∀ x : atom, x ∉ L → lc_td (A ^a^
 Inductive closed_td (d: aset) (a: transducer): Prop :=
 | closed_td_: lc_td a -> td_fv a ⊆ d -> closed_td d a.
 
+(* This measure function is used to guarantee termination of the denotation.
+Instead of addtion, we can also use [max] for the subterms. *)
+Fixpoint td_measure (a: transducer) : nat :=
+  match a with
+  | tdId => 1
+  | ⟨ _ | _ ⟩/id | ⟨ _ | _ ⟩/⟨ _ | _ | _ ⟩ => 1
+  | a1 ○ a2 | tdUnion a1 a2 => 1 + td_measure a1 + td_measure a2
+  | tdEx _ _ a => 1 + td_measure a
+  end.
+
+Lemma td_measure_gt_0 ρ : td_measure ρ > 0.
+Proof.
+  induction ρ; simpl; lia.
+Qed.
+
+Lemma td_measure_S ρ : exists n, td_measure ρ = S n.
+Proof.
+  destruct (Nat.lt_exists_pred 0 (td_measure ρ)).
+  pose proof (td_measure_gt_0 ρ). lia.
+  intuition eauto.
+Qed.
+
+Lemma open_preserves_td_measure ρ: forall k t,
+    td_measure ρ = td_measure ({k ~a> t} ρ).
+Proof.
+  induction ρ; simpl; eauto.
+Qed.
+
+Lemma subst_preserves_td_measure ρ: forall x t,
+    td_measure ρ = td_measure ({x:=t}a ρ).
+Proof.
+  induction ρ; simpl; eauto.
+Qed.
 
