TransducerProp.v
@@ -22,6 +22,14 @@ Import Transducer.
 
 (** * subst *)
 
+Ltac my_simplify_map :=
+  (repeat match goal with
+     | [H: context [ _ ∪ ∅ ] |- _ ] => setoid_rewrite map_union_empty in H
+     | [H: _ |- context [ _ ∪ ∅ ] ] => setoid_rewrite map_union_empty
+     | [H: context [ insert _ _ ∅ ] |- _ ] => setoid_rewrite insert_empty in H
+     | [H: _ |- context [ insert _ _ ∅  ] ] => setoid_rewrite insert_empty
+     end).
+
 Lemma subst_commute_td : forall x u_x y u_y a,
     x <> y -> x ∉ fv_value u_y -> y ∉ fv_value u_x ->
     {x := u_x }a ({y := u_y }a a) = {y := u_y }a ({x := u_x }a a).
@@ -54,8 +62,9 @@ Lemma open_fv_td' (a : transducer) (v : value): forall k,
   td_fv a ⊆ td_fv ({k ~a> v} a).
 Proof.
   pose open_fv_qualifier'.
-  induction a; intros; simpl; eauto.
-Admitted.
+  pose open_fv_value'.
+  induction a; intros; simpl; eauto; my_set_solver.
+Qed.
 
 Lemma open_subst_same_td: forall x y (a : transducer) k,
     x # a ->
@@ -67,8 +76,12 @@ Proof.
   repeat
     match goal with
     | H : forall k, _ # _ -> _ =_ |- _ => rewrite H by my_set_solver; eauto
+    | H : forall k, _ ∉ _ -> _ =_ |- _ => rewrite H by my_set_solver; eauto
     end.
-Admitted.
+  - rewrite open_subst_same_qualifier by my_set_solver.
+    repeat rewrite open_subst_same_value by my_set_solver. eauto.
+  - rewrite open_subst_same_qualifier by my_set_solver. eauto.
+Qed.
 
 Lemma subst_open_td: forall (a: transducer) (x:atom) (u: value) (w: value) (k: nat),
     lc w -> {x := w}a ({k ~a> u} a) = ({k ~a> {x := w}v u} ({x := w}a a)).
@@ -80,7 +93,10 @@ Proof.
     match goal with
     | H : context [lc _ -> _] |- _ => rewrite H by my_set_solver; eauto
     end.
-Admitted.
+  - rewrite subst_open_qualifier by my_set_solver.
+    repeat rewrite subst_open_value by my_set_solver. eauto.
+  - rewrite subst_open_qualifier by my_set_solver. eauto.
+Qed.
 
 Lemma subst_open_td_closed:
   ∀ (a : transducer) (x : atom) (u w : value) (k : nat),
@@ -116,21 +132,52 @@ Lemma fv_of_subst_td_closed:
     closed_value u ->
     td_fv ({x := u }a a) = (td_fv a ∖ {[x]}).
 Proof.
-  induction a; simpl; eauto using fv_of_subst_qualifier_closed.
-Admitted.
+  induction a; simpl; intros; eauto;
+    repeat
+      match goal with
+      | H : closed_value _ -> td_fv _ = _ |- _ => rewrite H by my_set_solver; eauto
+      end;
+    repeat rewrite fv_of_subst_qualifier_closed by eauto;
+    repeat rewrite fv_of_subst_value_closed by eauto;
+    my_set_solver.
+Qed.
 
-Lemma open_not_in_eq_td (x : atom) (a : transducer) k :
+Lemma open_not_in_eq_td (x : atom) (a : transducer): forall k,
   x # {k ~a> x} a ->
   forall e, a = {k ~a> e} a.
 Proof.
-  induction a; simpl; intros; eauto.
-  f_equal. eapply open_not_in_eq_qualifier. my_set_solver.
-  (* all: f_equal; auto_apply; my_set_solver. *)
-Admitted.
+  induction a; simpl; intros; eauto; f_equal;
+        try (rewrite <- (open_not_in_eq_qualifier x) by my_set_solver; eauto);
+        try (rewrite <- (open_not_in_eq_value x) by my_set_solver; eauto);
+        try (auto_apply; my_set_solver).
+Qed.
+
+Lemma lc_subst_phi1:
+  forall x (u: value) (ϕ: qualifier), lc_phi1 ({x := u}q ϕ) -> lc u -> lc_phi1 ϕ.
+Proof.
+  unfold lc_phi1. intros. simp_hyps.
+  auto_exists_L. intros.
+  ospecialize * H. my_set_solver.
+  rewrite <- subst_open_var_qualifier in H by my_set_solver.
+  eauto using lc_subst_qualifier.
+Qed.
+
+Lemma lc_subst_phi2:
+  forall x (u: value) (ϕ: qualifier), lc_phi2 ({x := u}q ϕ) -> lc u -> lc_phi2 ϕ.
+Proof.
+  unfold lc_phi2. intros. simp_hyps.
+  auto_exists_L. intros.
+  ospecialize * (H x0 _ y). my_set_solver. my_set_solver.
+  repeat rewrite <- subst_open_var_qualifier in H by my_set_solver.
+  apply lc_subst_qualifier in H; eauto.
+Qed.
 
 Lemma lc_subst_td:
   forall x (u: value) (a: transducer), lc_td ({x := u}a a) -> lc u -> lc_td a.
 Proof.
+  pose lc_subst_phi1.
+  pose lc_subst_phi2.
+  pose lc_subst_value.
   intros.
   remember (({x:=u}a) a).
   generalize dependent a.
@@ -138,11 +185,10 @@ Proof.
       match goal with
       | H : _ = {_:=_}a ?a |- _ => destruct a; simpl in *; simplify_eq
       end; eauto using lc_td.
-  econstructor.
-  (* auto_exists_L_intros. specialize_with x0. specialize_with y. *)
-  (* rewrite <- !subst_open_var_qualifier in H by (eauto; my_set_solver). *)
-  (* eauto using lc_subst_qualifier. *)
-Admitted.
+  - auto_exists_L. intros x0 Hx0. repeat specialize_with x0.
+    auto_apply; eauto.
+    rewrite <- subst_open_var_td by my_set_solver. eauto.
+Qed.
 
 Lemma open_td_idemp: forall u (v: value) (a: transducer) (k: nat),
     lc v ->
@@ -155,10 +201,162 @@ Qed.
 
 Lemma subst_intro_td: ∀ (A: transducer) (x : atom) (w : value) (k : nat),
     x # A → lc w → ({x:=w}a) ({k ~a> x} A) = {k ~a> w} A.
-Admitted.
+Proof.
+  intros.
+  specialize (subst_open_td A x x w k) as J.
+  simpl in J. rewrite decide_True in J; auto.
+  rewrite J; auto. rewrite subst_fresh_td; auto.
+Qed.
+
+Lemma lc_phi1_body: ∀ n vals prop,
+    lc_phi1 (@qual n vals prop) -> Vector.Forall (fun v => body (treturn v)) vals.
+Proof.
+  intros. subst. sinvert H.
+  rewrite Vector.Forall_forall. intros.
+  auto_exists_L. intros.
+  ospecialize * (H0 x0). my_set_solver.
+  sinvert H0.
+  apply Classical_Prop.EqdepTheory.inj_pair2 in H4.
+  apply Classical_Prop.EqdepTheory.inj_pair2 in H5.
+  subst.
+  rewrite VectorSpec.Forall_map in H3.
+  rewrite Vector.Forall_forall in H3. eauto.
+Qed.
+
+Lemma lc_phi2_body: ∀ n vals prop,
+    lc_phi2 (@qual n vals prop) ->
+    Vector.Forall (fun v =>
+                     exists (L : aset), (forall (x : atom), x ∉ L -> forall (y : atom), y ∉ L -> lc ({0 ~v> y} ({1 ~v> x} v)))) vals.
+Proof.
+  intros. subst. sinvert H.
+  rewrite Vector.Forall_forall. intros.
+  auto_exists_L. intros.
+  ospecialize * (H0 x0 _ y). my_set_solver. my_set_solver.
+  sinvert H0.
+  apply Classical_Prop.EqdepTheory.inj_pair2 in H5.
+  apply Classical_Prop.EqdepTheory.inj_pair2 in H6.
+  subst.
+  repeat rewrite VectorSpec.Forall_map in H4.
+  rewrite Vector.Forall_forall in H4. eauto.
+Qed.
+
+Check Vector.In.
+
+(* NOTE: Very very annoying, a reverse version of map_ext, using classical logic *)
+Lemma vector_map_ext_in' {A B: Type} (f g: A -> B) {n: nat} (vec: vec A n):
+  vmap f vec = vmap g vec -> (forall x, @Vector.In A x n vec -> f x = g x).
+Proof.
+  induction vec; simpl; intros.
+  - inversion H0.
+  - sinvert H.
+    apply Classical_Prop.EqdepTheory.inj_pair2 in H3.
+    sinvert H0; eauto.
+    apply Classical_Prop.EqdepTheory.inj_pair2 in H5. subst.
+    eapply IHvec in H3; eauto.
+Qed.
+
+Check fact1_value.
+
+Lemma fact1_value_twice: forall (u v1 v2: value) (e: value) i j1 j2,
+    i <> j1 -> i <> j2 -> j1 <> j2 ->
+    {i ~v> u} ({j1 ~v> v1} ({j2 ~v> v2} e)) = {j1 ~v> v1} ({j2 ~v> v2} e) -> {i ~v> u} e = e.
+Proof.
+  intros.
+  assert ({i ~v> u} ({j2 ~v> v2} e) = {j2 ~v> v2} e).
+  apply fact1_value with (j := j1) (v:= v1); eauto.
+  apply fact1_value with (j := j2) (v:= v2); eauto.
+Qed.
+
+Lemma fact1_qualifier: forall (u v: value) (ϕ: qualifier) i j,
+    i <> j -> {i ~q> u} ({j ~q> v} ϕ) = {j ~q> v} ϕ -> {i ~q> u} ϕ = ϕ.
+Proof.
+  intros.
+  destruct ϕ. simpl. f_equal.
+  rewrite <- Vector.map_id.
+  apply Vector.map_ext_in.
+  simpl in H0. sinvert H0.
+  apply Classical_Prop.EqdepTheory.inj_pair2 in H2.
+  rewrite Vector.map_map in H2.
+  intros.
+  eapply vector_map_ext_in' in H2; eauto.
+  pose fact1_value; eauto.
+Qed.
+
+Lemma fact1_qualifier_twice: forall (u v1 v2: value) (ϕ: qualifier) i j1 j2,
+    i <> j1 -> i <> j2 -> j1 <> j2 ->
+    {i ~q> u} ({j1 ~q> v1} ({j2 ~q> v2} ϕ)) = {j1 ~q> v1} ({j2 ~q> v2} ϕ) -> {i ~q> u} ϕ = ϕ.
+Proof.
+  intros.
+  assert ({i ~q> u} ({j2 ~q> v2} ϕ) = {j2 ~q> v2} ϕ).
+  apply fact1_qualifier with (j := j1) (v:= v1); eauto.
+  apply fact1_qualifier with (j := j2) (v:= v2); eauto.
+Qed.
+
+Lemma open_rec_lc_phi1: ∀ (u : value) ϕ (k : nat), lc_phi1 ϕ -> {S k ~q> u} ϕ = ϕ.
+Proof.
+  intros. destruct ϕ. apply lc_phi1_body in H.
+  simpl. f_equal.
+  rewrite <- Vector.map_id.
+  apply Vector.map_ext_in.
+  intros.
+  rewrite Vector.Forall_forall in H.
+  ospecialize * H; eauto.
+  destruct H.
+  auto_pose_fv y.
+  apply fact1_value with (j := 0) (v:= y). lia.
+  rewrite open_rec_lc_value; eauto. apply H. my_set_solver.
+Qed.
+
+(* NOTE: Very very annoying, when qualifier has builtin 1 or 2 arguments. *)
+Lemma open_rec_lc_phi2: ∀ (u : value) ϕ (k : nat), lc_phi2 ϕ -> {S (S k) ~q> u} ϕ = ϕ.
+Proof.
+  intros. destruct ϕ. apply lc_phi2_body in H.
+  simpl. f_equal.
+  rewrite <- Vector.map_id.
+  apply Vector.map_ext_in.
+  intros.
+  rewrite Vector.Forall_forall in H.
+  ospecialize * H; eauto.
+  destruct H.
+  auto_pose_fv y1. auto_pose_fv y2.
+  ospecialize * (H y1 _ y2); eauto. my_set_solver. my_set_solver.
+  eapply (fact1_value_twice _ y1 y2 _ _ 0 1); eauto.
+  rewrite open_rec_lc_value; eauto.
+Qed.
+
+Lemma fact1_td: forall (u v: value) (A: transducer) i j,
+    i <> j -> {i ~a> u} ({j ~a> v} A) = {j ~a> v} A -> {i ~a> u} A = A.
+Proof.
+  pose fact1_value.
+  pose fact1_qualifier.
+  intros u v. induction A; simpl; intros; eauto; f_equal; simp_hyps; eauto.
+  { apply fact1_qualifier in H0; eauto. }
+  all: sinvert H0; apply fact1_qualifier in H2; eauto.
+Qed.
+
+Lemma open_rec_lc_td_aux (u : value) m: forall A (k : nat), td_measure A ≤ m -> lc_td A -> {k ~a> u} A = A.
+Proof.
+  pose open_rec_lc_phi1.
+  pose open_rec_lc_phi2.
+  induction m; simpl; intros A k Hm H; sinvert H; simpl in *; sinvert Hm; eauto;
+    f_equal; eauto; try (rewrite open_rec_lc_value; eauto);
+    try (rewrite IHm; eauto; lia).
+  - auto_pose_fv x. apply fact1_td with (j := 0) (v := x); eauto.
+    rewrite IHm; eauto. rewrite <- open_preserves_td_measure; eauto. apply H0. my_set_solver.
+  - auto_pose_fv x. apply fact1_td with (j := 0) (v := x); eauto.
+    rewrite IHm; eauto. rewrite <- open_preserves_td_measure; eauto. lia. apply H0. my_set_solver.
+Qed.
 
 Lemma open_rec_lc_td: ∀ (u : value) A (k : nat), lc_td A -> {k ~a> u} A = A.
-Admitted.
+Proof.
+  pose open_rec_lc_phi1.
+  pose open_rec_lc_phi2.
+  intros. generalize dependent k.
+  induction H; simpl; intros; auto; f_equal; eauto;
+    try (rewrite open_rec_lc_value; eauto).
+  - auto_pose_fv x. apply fact1_td with (j := 0) (v := x); eauto.
+    rewrite H0; eauto. my_set_solver.
+Qed.
 
 Lemma lc_tdEx_destruct: forall b ϕ A, lc_td (tdEx b ϕ A) <-> lc_phi1 ϕ /\ body_td A.
 Proof.
